more experiments

week2/problems/problem3.dfy
@@ -11,10 +11,12 @@ method GCD(a: int, b: int) returns (gcd: int)
     var y := b;
     
     while y > 0 // changed, since "decreases expression must be bounded below by 0 at end of loop iteration"
-        // TODO: Write loop invariant(s)
 
-        
-        
+        invariant x >= 1
+        invariant y >= 0
+        invariant trivial_gcd(a,b,1,1) == trivial_gcd(x,y,1,1)
+        // (see pg 19, CSUR14.pdf - this problem has been fully outlined)
+
         decreases y
     {
         var temp := y;
@@ -24,3 +26,35 @@ method GCD(a: int, b: int) returns (gcd: int)
     
     gcd := x;
 }
+
+// inspired by the upcoming problems, i will use Helper Function(s)
+
+
+function min(a:int, b:int): int
+{
+    if a < b then a else b
+}
+
+
+// the following is a trivial implementation of gcd which is tail recursive
+// (iterative, but dafny can verify via induction without needing invariants)
+
+function trivial_gcd(a: int, b: int, gcd: int, k: int): int
+  requires a >= 0 && b >= 0
+  requires k > 0 && gcd > 0
+  requires k <= min(a, b) + 1
+  ensures trivial_gcd(a, b, gcd, k) > 0
+  decreases min(a, b) - k + 1
+{
+  if k <= min(a, b) then
+    if a % k == 0 && b % k == 0 then
+      trivial_gcd(a, b, k, k+1)
+    else
+      trivial_gcd(a, b, gcd, k+1)
+  else
+    gcd
+}
+
+lemma 
+
+
