week2/problems/problem4.dfy
@@ -14,14 +14,31 @@ method FastPower(base: int, exp: int) returns (result: int)
         invariant n >= 0
 
         invariant Power(base, exp) == Power(x, n) * result
+        // i think this invariant should be correct, it's not getting verified (checked with Smayan) - dafny keeps 
+        // saying that it is not maintained. after including the lemma (see later), it is working.
+
+        // i used a couple of examples as dry runs and noticed the pattern to arrive at this invariant which holds at
+        // initialization, maintainance and termination. nothing clever...
         
         decreases n
     {
+        PowerEven(x, n/2);
+        // including this lemma is super necessary. it helps in the verification of the invariant during maintanance.
+        // why? at the start of the loop dafny checks that if Power(base, exp) == Power(x, n) * result
+        // (contd. at end of loop body)
+        
         if n % 2 == 1 {
             result := result * x;
         }
+ 
         x := x * x;
         n := n / 2;
+
+        // as per the variable updates above, to check maintanance, dafny now checks if Power(base, exp) == Power(x*x, n/2) * result
+        // the implicit assumption here is that Power(x,n) == Power(x*x, n/2). We know this to be true as per the law of
+        // exponents, but dafny is unable to unfold the recursion of the Power() function to verify this property.
+        
+        // including the lemma in the loop body helps dafny utilise the property when verifying invariant maintanance.
     }
 }
 
@@ -30,4 +47,16 @@ function Power(base: int, exp: int): int
     requires exp >= 0
 {
     if exp == 0 then 1 else base * Power(base, exp - 1)
+}
+
+
+// [AI Disclosure] AI assistance was needed to figue this out
+lemma PowerEven(x: int, n: int)
+    requires n >= 0
+    ensures Power(x, 2 * n) == Power(x * x, n)
+{
+    if n == 0 { // base case, 1 == 1
+    } else {
+        PowerEven(x, n - 1); // inductive hypothesis, induction step done implictly by dafny
+    }
 }
