week2/problems/problem5.dfy
@@ -10,6 +10,8 @@ method ReverseNumber(n: int) returns (rev: int)
     
     while num > 0
         // TODO: Write loop invariant(s)
+
+        
         decreases num
     {
         var digit := num % 10;
